WIP - proving ForgetMemory

coq/proof/SoundForgetMemory.v
@@ -50,44 +50,107 @@ Inductive mem_change : Type :=
 (*   | None => None *)
 (*   end. *)
 
-Inductive mem_change_inject mi: mem_change -> mem_change -> Prop :=
+Inductive mem_change_inject conf_src conf_tgt invmem: mem_change -> mem_change -> Prop :=
 | mem_change_inject_alloc_alloc
-    gsz gn a
-  : mem_change_inject mi (mem_change_alloc gsz gn a) (mem_change_alloc gsz gn a)
+    gsz gn0 gn1 a
+    (N_INJECT: genericvalues_inject.gv_inject invmem.(InvMem.Rel.inject) gn0 gn1)
+  : mem_change_inject conf_src conf_tgt invmem (mem_change_alloc gsz gn0 a) (mem_change_alloc gsz gn1 a)
 | mem_change_inject_alloc_none
     gsz gn a
-  : mem_change_inject mi (mem_change_alloc gsz gn a) mem_change_none
+  : mem_change_inject conf_src conf_tgt invmem (mem_change_alloc gsz gn a) mem_change_none
 | mem_change_inject_none_alloc
     gsz gn a
-  : mem_change_inject mi mem_change_none (mem_change_alloc gsz gn a)
-| mem_change_inject_store
+  : mem_change_inject conf_src conf_tgt invmem mem_change_none (mem_change_alloc gsz gn a)
+| mem_change_inject_store_store
     ptr0 ptr1 gv0 gv1 ty a
-    (PTR_INJECT: genericvalues_inject.gv_inject mi ptr0 ptr1)
-    (VAL_INJECT: genericvalues_inject.gv_inject mi gv0 gv1)
-  : mem_change_inject mi (mem_change_store ptr0 ty gv0 a) (mem_change_store ptr1 ty gv1 a)
+    (PTR_INJECT: genericvalues_inject.gv_inject invmem.(InvMem.Rel.inject) ptr0 ptr1)
+    (VAL_INJECT: genericvalues_inject.gv_inject invmem.(InvMem.Rel.inject) gv0 gv1)
+  : mem_change_inject conf_src conf_tgt invmem (mem_change_store ptr0 ty gv0 a) (mem_change_store ptr1 ty gv1 a)
+| mem_change_inject_store_nop
+    ptr gv ty a b ofs
+    (GV2PTR: GV2ptr conf_src.(CurTargetData) (getPointerSize conf_tgt.(CurTargetData)) ptr = Some (Values.Vptr b ofs))
+    (IN: In b invmem.(InvMem.Rel.src).(InvMem.Unary.private))
+  : mem_change_inject conf_src conf_tgt invmem (mem_change_store ptr ty gv a) mem_change_none
 | mem_change_inject_free
     ptr0 ptr1
-    (PTR_INJECT: genericvalues_inject.gv_inject mi ptr0 ptr1)
-    : mem_change_inject mi (mem_change_free ptr0) (mem_change_free ptr1)
+    (PTR_INJECT: genericvalues_inject.gv_inject invmem.(InvMem.Rel.inject) ptr0 ptr1)
+    : mem_change_inject conf_src conf_tgt invmem (mem_change_free ptr0) (mem_change_free ptr1)
 | mem_change_inject_none
-    : mem_change_inject mi mem_change_none mem_change_none
+    : mem_change_inject conf_src conf_tgt invmem mem_change_none mem_change_none
 .
 
-Inductive mem_change_location conf st invst: mem_change -> option Ptr.t -> Prop :=
-| mem_change_location_alloc
-    bsz gn a
-  : mem_change_location conf st invst (mem_change_alloc bsz gn a) None
-| mem_change_location_store
-    ptr gv_ptr gv a
-    (STORE_PTR: InvState.Unary.sem_valueT conf st invst ptr.(fst) = Some gv_ptr)
-  : mem_change_location conf st invst (mem_change_store gv_ptr ptr.(snd) gv a) (Some ptr)
-| mem_change_location_free
-    ptr gv_ptr
-    (FREE_PTR: InvState.Unary.sem_valueT conf st invst ptr.(fst) = Some gv_ptr)
-  : mem_change_location conf st invst (mem_change_free gv_ptr) (Some ptr)
-| mem_change_location_none
-  : mem_change_location conf st invst mem_change_none None
-.
+(* Inductive mem_change_rel conf st: mem_change -> cmd -> Prop := *)
+(* | mem_change_rel_alloca *)
+(*     id ty v *)
+(*     tsz gn a *)
+(*     (TYPE: getTypeAllocSize conf.(CurTargetData) ty = Some tsz) *)
+(*     (VAL: getOperandValue conf.(CurTargetData) v st.(EC).(Locals) conf.(Globals)) *)
+(*   : mem_change_rel conf st (mem_change_alloc tsz gn a) (insn_alloca id ty v a) *)
+(* | mem_change_rel_malloc *)
+(*     id ty v *)
+(*     tsz gn a *)
+(*     (TYPE: getTypeAllocSize conf.(CurTargetData) ty = Some tsz) *)
+(*     (VAL: getOperandValue conf.(CurTargetData) v st.(EC).(Locals) conf.(Globals)) *)
+(*   : mem_change_rel conf st (mem_change_alloc tsz gn a) (insn_malloc id ty v a) *)
+(* | mem_change_rel_store *)
+(*     v_val gv_val *)
+(*     v_ptr gv_ptr *)
+(*     ty a sid *)
+(*     (VAL: getOperandValue conf.(CurTargetData) v_val st.(EC).(Locals) conf.(Globals) = Some gv_val) *)
+(*     (PTR: getOperandValue conf.(CurTargetData) v_ptr st.(EC).(Locals) conf.(Globals) = Some gv_ptr) *)
+(*   : mem_change_rel conf st (mem_change_store gv_ptr ty gv_val a) *)
+(*                    (insn_store sid ty v_val v_ptr a) *)
+(* | mem_change_rel_free *)
+(*     v_ptr gv_ptr fid ty *)
+(*     (PTR: getOperandValue conf.(CurTargetData) v_ptr st.(EC).(Locals) conf.(Globals) = Some gv_ptr) *)
+(*   : mem_change_rel conf st (mem_change_free gv_ptr) (insn_free fid ty v_ptr). *)
+(* | mem_change_rel_none *)
+(*     cmd *)
+(*     (NON_ALLOCA =  *)
+(*   : mem_change_rel conf st mem_change_none cmd *)
+
+Definition mem_change_rel conf st mc cmd: Prop :=
+  match cmd with
+  | insn_alloca _ ty v a =>
+    exists tsz gn,
+    <<TYPE: getTypeAllocSize conf.(CurTargetData) ty = Some tsz>> /\
+    <<VAL: getOperandValue conf.(CurTargetData) v st.(EC).(Locals) conf.(Globals) = Some gn>> /\
+    <<MEM_CH: mc = mem_change_alloc tsz gn a>>
+  | insn_malloc _ ty v a =>
+    exists tsz gn,
+    <<TYPE: getTypeAllocSize conf.(CurTargetData) ty = Some tsz>> /\
+    <<VAL: getOperandValue conf.(CurTargetData) v st.(EC).(Locals) conf.(Globals) = Some gn>> /\
+    <<MEM_CH: mc = mem_change_alloc tsz gn a>>
+  | insn_store _ ty v_val v_ptr a =>
+    exists gv_val gv_ptr,
+    <<VAL: getOperandValue conf.(CurTargetData) v_val st.(EC).(Locals) conf.(Globals) = Some gv_val>> /\
+    <<PTR: getOperandValue conf.(CurTargetData) v_ptr st.(EC).(Locals) conf.(Globals) = Some gv_ptr>> /\
+    <<MEM_CH: mc = mem_change_store gv_ptr ty gv_val a>>
+  | insn_free _ _ v_ptr =>
+    exists gv_ptr,
+    <<PTR: getOperandValue conf.(CurTargetData) v_ptr st.(EC).(Locals) conf.(Globals) = Some gv_ptr>> /\
+    <<MEM_CH: mc = mem_change_free gv_ptr>>
+  | _ => mc = mem_change_none
+  end.
+
+Definition mem_change_rel2 conf st mc cmd: Prop :=
+  match cmd with
+  | insn_alloca _ ty v a =>
+    exists tsz gn,
+    <<MEM_CH: mc = mem_change_alloc tsz gn a>>
+  | insn_malloc _ ty v a =>
+    exists tsz gn,
+    <<MEM_CH: mc = mem_change_alloc tsz gn a>>
+  | insn_store _ ty _ v_ptr a =>
+    exists gv_val gv_ptr,
+    <<PTR: getOperandValue conf.(CurTargetData) v_ptr st.(EC).(Locals) conf.(Globals) = Some gv_ptr>> /\
+    <<MEM_CH: mc = mem_change_store gv_ptr ty gv_val a>>
+  | insn_free _ _ v_ptr =>
+    exists gv_ptr,
+    <<PTR: getOperandValue conf.(CurTargetData) v_ptr st.(EC).(Locals) conf.(Globals) = Some gv_ptr>> /\
+    <<MEM_CH: mc = mem_change_free gv_ptr>>
+  | _ => mc = mem_change_none
+  end.
 
 Inductive mem_change_equiv (conf:Config) (mem0 mem1:mem): mem_change -> Prop :=
 | mem_change_equiv_alloc
@@ -103,7 +166,7 @@ Inductive mem_change_equiv (conf:Config) (mem0 mem1:mem): mem_change -> Prop :=
     (FREE: Some mem1 = free conf.(CurTargetData) mem0 ptr)
   : mem_change_equiv conf mem0 mem1 (mem_change_free ptr)
 | mem_change_equiv_none
-    (MEM: mem0 = mem1)
+    (MEM_EQ: mem0 = mem1)
   : mem_change_equiv conf mem0 mem1 mem_change_none
 .
 
@@ -123,46 +186,93 @@ Definition unique_preserved_mem conf st inv: Prop :=
 (*   | None => None *)
 (*   end. *)
 
-Lemma forget_memory_unary_sound1
-      conf st0 invst0 invmem0 inv0
-      def_memory st1 public gmax mem_change
-        (STATE: InvState.Unary.sem conf st0 invst0 invmem0 inv0)
-        (MEM: InvMem.Unary.sem conf gmax public st0.(Mem) invmem0)
-        (MEM_EQUIV: state_equiv_except_mem conf st0 st1 mem_change)
-        (MEM_CHANGE: mem_change_location conf st0 invst0 mem_change (Some def_memory))
-        (UNIQUE_PRSV: unique_preserved_mem conf st1 inv0)
-    : <<STATE_UNARY: InvState.Unary.sem conf st1 invst0 invmem0 (ForgetMemory.unary def_memory inv0)>> /\
-      <<MEM_UNARY: InvMem.Unary.sem conf gmax public st1.(Mem) invmem0>>.
-Proof.
-Admitted.
-
-Lemma forget_memory_unary_sound2
-      conf st0 st1 mem_change
-      invst0 invmem0 inv0 gmax public
-      (MEM: InvMem.Unary.sem conf gmax public st0.(Mem) invmem0)
-      (MEM_EQUIV : state_equiv_except_mem conf st0 st1 mem_change)
-      (MEM_CHANGE : mem_change_location conf st0 invst0 mem_change None)
-      (TGT : InvState.Unary.sem conf st0 invst0 invmem0 inv0)
-  : <<STATE_UNARY: InvState.Unary.sem conf st1 invst0 invmem0 inv0>> /\
-    <<MEM_UNARY: InvMem.Unary.sem conf gmax public st1.(Mem) invmem0>>.
-Proof.
-Admitted.
-
 Lemma some_injective A (a b:A):
   Some a = Some b -> a = b.
 Proof.
   congruence.
 Qed.
 
+(* monotonic feature of ForgetMemory *)
+
+Lemma not_in_maydiff_forget_memory_monotone
+      def_mem_src def_mem_tgt inv0 v
+      (NOT_MD: Invariant.not_in_maydiff (ForgetMemory.t def_mem_src def_mem_tgt inv0) v = true)
+  : Invariant.not_in_maydiff inv0 v = true.
+Proof.
+  unfold Invariant.not_in_maydiff in *.
+  unfold ForgetMemory.t in *.
+  destruct def_mem_tgt; destruct def_mem_src; ss.
+Qed.
+
+Lemma ExprPairSet_forget_memory_monotone
+      ep def_mem inv0
+      (INJECT: ExprPairSet.mem ep (Invariant.lessdef (ForgetMemory.unary def_mem inv0)) = true)
+  : ExprPairSet.mem ep (Invariant.lessdef inv0) = true.
+Proof.
+  unfold ForgetMemory.unary in *.
+  des_ifs. ss.
+  rewrite ExprPairSetFacts.filter_b in *; try by solve_compat_bool.
+  rewrite andb_true_iff in *. des. eauto.
+Qed.
+
+Lemma inject_value_forget_memory_monotone
+      v1 def_mem_src
+      v2 def_mem_tgt
+      inv0
+      (INJECT: Invariant.inject_value
+                 (ForgetMemory.t def_mem_src def_mem_tgt inv0) v1 v2)
+  : Invariant.inject_value inv0 v1 v2.
+Proof.
+  unfold Invariant.inject_value in *.
+  unfold is_true in *.
+  repeat rewrite orb_true_iff in INJECT.
+  repeat rewrite orb_true_iff.
+  des.
+  - left. left. left.
+    solve_des_bool.
+    apply andb_true_iff; split; eauto using not_in_maydiff_forget_memory_monotone.
+  - left. left. right.
+    solve_des_bool.
+    apply andb_true_iff; split; eauto using not_in_maydiff_forget_memory_monotone.
+    destruct def_mem_src; destruct def_mem_tgt; ss;
+      eapply ExprPairSet_forget_memory_monotone; eauto.
+  - left. right.
+    solve_des_bool.
+    apply andb_true_iff; split; eauto using not_in_maydiff_forget_memory_monotone.
+    destruct def_mem_src; destruct def_mem_tgt; ss;
+      eapply ExprPairSet_forget_memory_monotone; eauto.
+  - right.
+    rewrite <- ExprPairSetFacts.exists_iff in *;try by solve_compat_bool.
+    unfold ExprPairSet.Exists in *. des.
+    apply InvState.get_rhs_in_spec in INJECT. des.
+    esplits.
+    + eapply InvState.get_rhs_in_spec2; eauto.
+      destruct def_mem_src; destruct def_mem_tgt; ss;
+        rewrite ExprPairSetFacts.mem_iff in *;
+        eapply ExprPairSet_forget_memory_monotone; eauto.
+    + solve_des_bool.
+      apply andb_true_iff.
+      split.
+      * destruct def_mem_src; destruct def_mem_tgt; ss;
+          rewrite ExprPairSetFacts.mem_iff in *;
+          eapply ExprPairSet_forget_memory_monotone; eauto.
+      * unfold Invariant.not_in_maydiff_expr in *.
+        apply forallb_forall. i.
+        eapply forallb_forall in INJECT2; eauto.
+        eapply not_in_maydiff_forget_memory_monotone; eauto.
+Qed.
+
+(* soundness *)
+
 Lemma mem_inject_change
       conf_src mem0_src mem1_src mem_change_src
       conf_tgt mem0_tgt mem1_tgt mem_change_tgt
-      mi
+      invmem0
       (MEM_CHANGE_EQUIV_SRC : mem_change_equiv conf_src mem0_src mem1_src mem_change_src)
       (MEM_CHANGE_EQUIV_TGT : mem_change_equiv conf_tgt mem0_tgt mem1_tgt mem_change_tgt)
-      (MEM_CHANGE_INJECT : mem_change_inject mi mem_change_src mem_change_tgt)
-      (INJECT : Memory.Mem.inject mi mem0_src mem0_tgt)
-  : Memory.Mem.inject mi mem1_src mem1_tgt.
+      (MEM_CHANGE_INJECT : mem_change_inject conf_src conf_tgt invmem0 mem_change_src mem_change_tgt)
+      (INJECT : Memory.Mem.inject invmem0.(InvMem.Rel.inject) mem0_src mem0_tgt)
+  : Memory.Mem.inject invmem0.(InvMem.Rel.inject) mem1_src mem1_tgt.
 Proof.
   inv MEM_CHANGE_INJECT.
   - inv INJECT. inv MEM_CHANGE_EQUIV_SRC. inv MEM_CHANGE_EQUIV_TGT.
@@ -246,17 +356,210 @@ Proof.
     (*   memory_sim.MoreMem.mem_inj *)
     admit. (* store - store *)
   - inv MEM_CHANGE_EQUIV_SRC. inv MEM_CHANGE_EQUIV_TGT.
+    unfold mstore in *. des_ifs.
+    admit. (* store to private *)
+    
+  - inv MEM_CHANGE_EQUIV_SRC. inv MEM_CHANGE_EQUIV_TGT.
     unfold free in *. des_ifs.
     eapply Memory.Mem.free_left_inject; eauto.
     eapply Memory.Mem.free_right_inject; eauto.
     admit. (* free - free *)
   - inv MEM_CHANGE_EQUIV_SRC. inv MEM_CHANGE_EQUIV_TGT.
-    econs; eauto.
+    eauto.
+Admitted.
+
+Lemma forget_memory_maydiff_preserved
+      conf_src st0_src st1_src mem_change_src def_mem_src
+      conf_tgt st0_tgt st1_tgt mem_change_tgt def_mem_tgt
+      invst0 invmem0 inv0
+      (MEM_EQUIV_SRC : state_equiv_except_mem conf_src st0_src st1_src mem_change_src)
+      (MEM_EQUIV_TGT : state_equiv_except_mem conf_tgt st0_tgt st1_tgt mem_change_tgt)
+      (MAYDIFF : forall id : Tag.t * id,
+          IdTSet.mem id (Invariant.maydiff inv0) = false ->
+          InvState.Rel.sem_inject st0_src st0_tgt invst0 (InvMem.Rel.inject invmem0) id)
+  : <<RES: forall id : Tag.t * id,
+      IdTSet.mem id (Invariant.maydiff (ForgetMemory.t def_mem_src def_mem_tgt inv0)) = false ->
+      InvState.Rel.sem_inject st1_src st1_tgt invst0 (InvMem.Rel.inject invmem0) id>>.
+Proof.
+  ii.
+  assert (DROP_FORGET_MEMORY:IdTSet.mem id0 (Invariant.maydiff inv0) = false).
+  { destruct def_mem_src; destruct def_mem_tgt; ss. }
+  exploit MAYDIFF; eauto.
+  { inv MEM_EQUIV_SRC.
+    unfold InvState.Unary.sem_idT in *.
+    destruct id0 as [[] x]; eauto.
+    ss. rewrite LOCALS_EQ. eauto.
+  }
+  i. des.
+  esplits; eauto.
+  inv MEM_EQUIV_TGT.
+  unfold InvState.Unary.sem_idT in *.
+  destruct id0 as [[] x]; eauto.
+  ss. rewrite <- LOCALS_EQ. eauto.
+Qed.
+
+Lemma sem_idT_eq_locals
+      st0 st1 invst0 x gv
+      (SEM_IDT: InvState.Unary.sem_idT st1 invst0 x = Some gv)
+      (LOCALS_EQ : Locals (EC st0) = Locals (EC st1))
+  : InvState.Unary.sem_idT st0 invst0 x = Some gv.
+Proof.
+  destruct x as [[] x]; unfold InvState.Unary.sem_idT in *; ss.
+  rewrite LOCALS_EQ; eauto.
+Qed.    
+
+Lemma sem_valueT_eq_locals
+      conf st0 st1 invst0 v gv
+      (SEM_EXPR: InvState.Unary.sem_valueT conf st0 invst0 v = Some gv)
+      (LOCALS_EQ: Locals (EC st0) = Locals (EC st1))
+  : InvState.Unary.sem_valueT conf st1 invst0 v = Some gv.
+Proof.
+  destruct v; eauto.
+  eapply sem_idT_eq_locals; eauto.
+Qed.
+
+Lemma sem_list_valueT_eq_locals
+      conf st0 st1 invst0 lsv lgv
+      (SEM_EXPR: InvState.Unary.sem_list_valueT conf st0 invst0 lsv = Some lgv)
+      (LOCALS_EQ: Locals (EC st0) = Locals (EC st1))
+  : InvState.Unary.sem_list_valueT conf st1 invst0 lsv = Some lgv.
+Proof.
+  revert lgv SEM_EXPR.
+  induction lsv; ss; i.
+  des_ifs.
+  - exploit IHlsv; eauto. i.
+    symmetry in LOCALS_EQ.
+    exploit sem_valueT_eq_locals; eauto. i. clarify.
+  - exploit IHlsv; eauto. i.
+    clarify.
+  - exploit sem_valueT_eq_locals; eauto. i. clarify.
+Qed.
+
+Ltac sem_valueT_congruence :=
+      repeat
+        match goal with
+        | [H1: InvState.Unary.sem_valueT ?conf ?st1 ?invst ?v = Some ?gv1,
+               H2: InvState.Unary.sem_valueT ?conf ?st2 ?invst ?v = _,
+                   LOCALS: Locals (EC ?st1) = Locals (EC ?st2) |- _] =>
+          erewrite sem_valueT_eq_locals in H2; try exact H1; try exact LOCALS; inv H2
+        | [H1: InvState.Unary.sem_list_valueT ?conf ?st1 ?invst ?lsv = Some ?lgv,
+               H2: InvState.Unary.sem_list_valueT ?conf ?st2 ?invst ?lsv = _,
+                   LOCALS: Locals (EC ?st1) = Locals (EC ?st2) |- _] =>
+          erewrite sem_list_valueT_eq_locals in H2; try exact H1; try exact LOCALS; inv H2
+        end;
+      eauto; try congruence.
+
+Lemma sem_expr_eq_locals_mem
+      conf st0 st1 invst0 e gv
+      (SEM_EXPR: InvState.Unary.sem_expr conf st0 invst0 e = Some gv)
+      (LOCALS_EQ: Locals (EC st0) = Locals (EC st1))
+      (MEM_EQ: Mem st0 = Mem st1)
+  : InvState.Unary.sem_expr conf st1 invst0 e = Some gv.
+Proof.
+  destruct e; ss;
+    des_ifs; sem_valueT_congruence; clarify.
+  eapply sem_valueT_eq_locals; eauto.
+Qed.
+
+Lemma unary_sem_eq_locals_mem
+      conf st0 st1 invst0 invmem0 inv0
+      (STATE: InvState.Unary.sem conf st0 invst0 invmem0 inv0)
+      (LOCALS_EQ: Locals (EC st0) = Locals (EC st1))
+      (MEM_EQ : Mem st0 = Mem st1)
+  : InvState.Unary.sem conf st1 invst0 invmem0 inv0.
+Proof.
+  inv STATE.
+  econs.
+  - ii.
+    exploit LESSDEF; eauto.
+    { eapply sem_expr_eq_locals_mem; eauto. }
+    i. des.
+    esplits; eauto.
+    exploit sem_expr_eq_locals_mem; eauto.
+  - inv NOALIAS.
+    econs; i; [exploit DIFFBLOCK | exploit NOALIAS0]; eauto;
+      eapply sem_valueT_eq_locals; eauto.
+  - ii. exploit UNIQUE; eauto. intro UNIQ_X. inv UNIQ_X.
+    econs; try rewrite <- LOCALS_EQ; try rewrite <- MEM_EQ; eauto.
+  - ii. exploit PRIVATE; eauto.
+    eapply sem_idT_eq_locals; eauto.
+Qed.
+
+Lemma forget_memory_unary_sound1
+      conf st0 invst0 invmem0 inv0
+      cmd st1 public gmax mem_change def_memory
+      (STATE: InvState.Unary.sem conf st0 invst0 invmem0 inv0)
+      (DEF_MEM: Cmd.get_def_memory cmd = Some def_memory)
+      (MEM: InvMem.Unary.sem conf gmax public st0.(Mem) invmem0)
+      (MEM_EQUIV: state_equiv_except_mem conf st0 st1 mem_change)
+      (MEM_CHANGE: mem_change_rel2 conf st0 mem_change cmd)
+      (UNIQUE_PRSV: unique_preserved_mem conf st1 inv0)
+  : <<STATE_UNARY: InvState.Unary.sem conf st1 invst0 invmem0 (ForgetMemory.unary def_memory inv0)>> /\
+                   <<MEM_UNARY: InvMem.Unary.sem conf gmax public st1.(Mem) invmem0>>.
+Proof.
+  destruct mem_change;
+    try by (destruct cmd; ss; des; congruence).
+  - splits.
+    + inv STATE.
+      (* econs; eauto. *)
+      (* { ii. exploit LESSDEF; eauto. *)
+      admit. (* lessdef - should treat load *)
+    + inv MEM_EQUIV.
+      inv MEM_CHANGE_EQUIV.
+      inv MEM.
+      admit. (* mstore, mstore_aux *)
+  - splits.
+    + inv STATE.
+      (* econs. *)
+      (* { ii. *)
+      (*   exploit LESSDEF. *)
+      (*   { admit. (* in - monotone *) } *)
+      (*   { admit. (* sem_expr monotone? *) } *)
+      (*   i. des. *)
+      (*   esplits; eauto. *)
+      (*   admit. *)
+      (* } *)
+      admit.
+    + inv MEM_EQUIV.
+      inv MEM_CHANGE_EQUIV.
+      inv MEM.
+      unfold free in *. des_ifs.
+      econs; eauto.
+      * i. exploit PRIVATE; eauto. i. des.
+        split; eauto.
+        exploit Memory.Mem.valid_block_free_1; eauto.
+      * i. exploit PRIVATE_PARENT; eauto. i. des.
+        split; eauto.
+        exploit Memory.Mem.valid_block_free_1; eauto.
+      *  i. exploit MEM_PARENT; eauto.
+         admit. (* should handle mload_aux *)
+Admitted.
+
+Lemma forget_memory_unary_sound2
+      conf st0 st1 mem_change
+      cmd invst0 invmem0 inv0 gmax public
+      (STATE: InvState.Unary.sem conf st0 invst0 invmem0 inv0)
+      (DEF_MEM: Cmd.get_def_memory cmd = None)
+      (MEM: InvMem.Unary.sem conf gmax public st0.(Mem) invmem0)
+      (MEM_EQUIV : state_equiv_except_mem conf st0 st1 mem_change)
+      (MEM_CHANGE : mem_change_rel2 conf st0 mem_change cmd)
+      (UNIQUE_PRSV: unique_preserved_mem conf st1 inv0)
+  : <<STATE_UNARY: InvState.Unary.sem conf st1 invst0 invmem0 inv0>> /\
+    <<MEM_UNARY: InvMem.Unary.sem conf gmax public st1.(Mem) invmem0>>.
+Proof.
+  destruct mem_change.
+  - admit.
+  - destruct cmd; ss; des; congruence.
+  - destruct cmd; ss; des; congruence.
+  - inv MEM_EQUIV. inv MEM_CHANGE_EQUIV.
+    rewrite <- MEM_EQ.
+    esplits; eauto.
+    eapply unary_sem_eq_locals_mem; eauto.
 Admitted.
 
 Lemma forget_memory_sound
-      conf_src st0_src st1_src def_memory_src mem_change_src
-      conf_tgt st0_tgt st1_tgt def_memory_tgt mem_change_tgt
+      conf_src st0_src st1_src mem_change_src cmd_src
+      conf_tgt st0_tgt st1_tgt mem_change_tgt cmd_tgt
       invst0 invmem0 inv0
       (STATE: InvState.Rel.sem conf_src conf_tgt st0_src st0_tgt invst0 invmem0 inv0)
       (MEM: InvMem.Rel.sem conf_src conf_tgt st0_src.(Mem) st0_tgt.(Mem) invmem0)
@@ -268,102 +571,180 @@ Lemma forget_memory_sound
                         conf_tgt
                         st0_tgt st1_tgt
                         mem_change_tgt)
-      (MEM_CHANGE_SRC: mem_change_location conf_src st0_src invst0.(InvState.Rel.src) mem_change_src def_memory_src)
-      (MEM_CHANGE_TGT: mem_change_location conf_tgt st0_tgt invst0.(InvState.Rel.tgt) mem_change_tgt def_memory_tgt)
-      (MEM_CHANGE_INJECT: mem_change_inject invmem0.(InvMem.Rel.inject) mem_change_src mem_change_tgt)
+      (MEM_CHANGE_SRC: mem_change_rel2 conf_src st0_src mem_change_src cmd_src)
+      (MEM_CHANGE_TGT: mem_change_rel2 conf_tgt st0_tgt mem_change_tgt cmd_tgt)
+      (MEM_CHANGE_INJECT: mem_change_inject conf_src conf_tgt invmem0 mem_change_src mem_change_tgt)
       (UNIQUE_PRSV_SRC: unique_preserved_mem conf_src st1_src inv0.(Invariant.src))
       (UNIQUE_PRSV_TGT: unique_preserved_mem conf_tgt st1_tgt inv0.(Invariant.tgt))
   : <<STATE: InvState.Rel.sem conf_src conf_tgt st1_src st1_tgt invst0 invmem0
-                              (ForgetMemory.t def_memory_src def_memory_tgt inv0) >> /\
+                              (ForgetMemory.t (Cmd.get_def_memory cmd_src) (Cmd.get_def_memory cmd_tgt) inv0) >> /\
     <<MEM: InvMem.Rel.sem conf_src conf_tgt st1_src.(Mem) st1_tgt.(Mem) invmem0>>.
 Proof.
-  inv STATE.
-  unfold ForgetMemory.t.
-  destruct def_memory_src as [[]|], def_memory_tgt as [[]|]; ss.
-  inv MEM.
+  inv STATE. inv MEM.
+  
+  destruct (Cmd.get_def_memory cmd_src) eqn:DEF_MEM_SRC;
+    destruct (Cmd.get_def_memory cmd_tgt) eqn:DEF_MEM_TGT.
+  - hexploit forget_memory_unary_sound1; try exact SRC; try exact DEF_MEM_SRC; eauto. i. des.
+    hexploit forget_memory_unary_sound1; try exact TGT; try exact DEF_MEM_TGT; eauto. i. des.
+    hexploit forget_memory_maydiff_preserved; try exact MAYDIFF; eauto. i. des.
+    inv MEM_EQUIV_SRC. inv MEM_EQUIV_TGT.
+    hexploit mem_inject_change; try exact MEM_CHANGE_INJECT; eauto. i.
+    esplits; econs; eauto.
+  - hexploit forget_memory_unary_sound1; try exact SRC; try exact DEF_MEM_SRC; eauto. i. des.
+    hexploit forget_memory_unary_sound2; try exact TGT; try exact DEF_MEM_TGT; eauto. i. des.
+    hexploit forget_memory_maydiff_preserved; try exact MAYDIFF; eauto. i. des.
+    inv MEM_EQUIV_SRC. inv MEM_EQUIV_TGT.
+    hexploit mem_inject_change; try exact MEM_CHANGE_INJECT; eauto. i.
+    esplits; econs; eauto.
+  - hexploit forget_memory_unary_sound2; try exact SRC; try exact DEF_MEM_SRC; eauto. i. des.
+    hexploit forget_memory_unary_sound1; try exact TGT; try exact DEF_MEM_TGT; eauto. i. des.
+    hexploit forget_memory_maydiff_preserved; try exact MAYDIFF; eauto. i. des.
+    inv MEM_EQUIV_SRC. inv MEM_EQUIV_TGT.
+    hexploit mem_inject_change; try exact MEM_CHANGE_INJECT; eauto. i.
+    esplits; econs; eauto.
+  - hexploit forget_memory_unary_sound2; try exact SRC; try exact DEF_MEM_SRC; eauto. i. des.
+    hexploit forget_memory_unary_sound2; try exact TGT; try exact DEF_MEM_TGT; eauto. i. des.
+    hexploit forget_memory_maydiff_preserved; try exact MAYDIFF; eauto. i. des.
+    inv MEM_EQUIV_SRC. inv MEM_EQUIV_TGT.
+    hexploit mem_inject_change; try exact MEM_CHANGE_INJECT; eauto. i.
+    esplits; econs; eauto.
+Qed.
+    
+(*     esplits. *)
+(*     + econs; eauto. *)
+(*       ss. i. *)
+(*       hexploit MAYDIFF; eauto. i. *)
+(*       ii. *)
+(*       i. *)
+(*       ss. eauto. *)
+(*       admit. *)
+(*     + econs; eauto. *)
+(*       eapply mem_inject_change; eauto. *)
+(*       * inv MEM_EQUIV_SRC; eauto. *)
+(*       * inv MEM_EQUIV_TGT; eauto. *)
+(*   - *)
+  
+(*   inv STATE. *)
+(*   destruct mem_change_src; destruct mem_change_tgt; inv MEM_CHANGE_INJECT. *)
+(*   - destruct cmd_src eqn:CMDSRC; destruct cmd_tgt eqn:CMDTGT; ss; des; *)
+(*       try congruence. *)
+(*     + inv MEM_CH; inv MEM_CH0. *)
+(*     +  *)
 
-  - exploit forget_memory_unary_sound1; try exact SRC; eauto. i. des.
-    exploit forget_memory_unary_sound1; try exact TGT; eauto. i. des.
-    splits.
-    + econs; ss; eauto. i.
-      hexploit MAYDIFF; eauto. i.
-      ii. exploit H.
-      { destruct id0 as [[]]; eauto.
-        inv MEM_EQUIV_SRC; solve_sem_idT.
-        rewrite -> LOCALS_EQ; eauto.
-      }
-      i. des.
-      esplits; eauto.
-      destruct id0 as [[]]; eauto.
-      inv MEM_EQUIV_TGT;
-        solve_sem_idT; rewrite <- LOCALS_EQ; eauto.
-    + econs; ss; eauto.
-      inv MEM_EQUIV_SRC.
-      inv MEM_EQUIV_TGT.
+(*     admit. (* alloc - alloc *) } *)
+(*   { admit. (* alloc - none *) } *)
+(*   { admit. (* store - store *) } *)
+(*   { admit. (* store - none *) } *)
+(*   { admit. (* free - free *) } *)
+(*   { admit. (* none - alloc *) } *)
+(*   { admit. (* none - none *) } *)
 
-      eapply mem_inject_change; eauto.
+
+  
+(*   destruct (Cmd.get_def_memory cmd_src) eqn:DEF_MEM_SRC; *)
+(*     destruct (Cmd.get_def_memory cmd_tgt) eqn:DEF_MEM_TGT. *)
+(*   - destruct cmd_src; destruct cmd_tgt; ss. *)
+(*     + admit. (* free - free *) *)
+(*     + admit. (* free - store : cont. *) *)
+(*     + admit. (* store - free : cont.  *) *)
+(*     + admit. (* store - store *) *)
+(*   - (* destruct cmd_src; destruct cmd_tgt; ss. *) *)
+(*     admit. *)
+(*   - admit. *)
+(*   - ss. *)
+(*     unfold mem_change_rel2 in *. *)
+(*     destruct cmd_src; destruct cmd_tgt; ss. *)
+
+
+
+
+  
+(*   unfold ForgetMemory.t. *)
+(*   destruct def_memory_src as [[]|], def_memory_tgt as [[]|]; ss. *)
+(*   inv MEM. *)
+
+(*   - exploit forget_memory_unary_sound1; try exact SRC; eauto. i. des. *)
+(*     exploit forget_memory_unary_sound1; try exact TGT; eauto. i. des. *)
+(*     splits. *)
+(*     + econs; ss; eauto. i. *)
+(*       hexploit MAYDIFF; eauto. i. *)
+(*       ii. exploit H. *)
+(*       { destruct id0 as [[]]; eauto. *)
+(*         inv MEM_EQUIV_SRC; solve_sem_idT. *)
+(*         rewrite -> LOCALS_EQ; eauto. *)
+(*       } *)
+(*       i. des. *)
+(*       esplits; eauto. *)
+(*       destruct id0 as [[]]; eauto. *)
+(*       inv MEM_EQUIV_TGT; *)
+(*         solve_sem_idT; rewrite <- LOCALS_EQ; eauto. *)
+(*     + econs; ss; eauto. *)
+(*       inv MEM_EQUIV_SRC. *)
+(*       inv MEM_EQUIV_TGT. *)
+
+(*       eapply mem_inject_change; eauto. *)
       
-  - inv MEM.
-    exploit forget_memory_unary_sound1; try exact SRC; eauto. i. des.
-    exploit forget_memory_unary_sound2; try exact TGT; eauto. i. des.
-    splits.
-    + econs; ss; eauto.
-      i.
-      hexploit MAYDIFF; eauto. i.
-      ii. exploit H.
-      { destruct id0 as [[]]; eauto.
-        inv MEM_EQUIV_SRC; solve_sem_idT.
-        rewrite -> LOCALS_EQ; eauto.
-      }
-      i. des.
-      esplits; eauto.
-      destruct id0 as [[]]; eauto.
-      inv MEM_EQUIV_TGT;
-        solve_sem_idT; rewrite <- LOCALS_EQ; eauto.
-    + econs; ss; eauto.
-      inv MEM_EQUIV_SRC.
-      inv MEM_EQUIV_TGT.
-      eapply mem_inject_change; eauto.
-  - inv MEM.
-    exploit forget_memory_unary_sound2; try exact SRC; eauto. i. des.
-    exploit forget_memory_unary_sound1; try exact TGT; eauto. i. des.
-    splits.
-    + econs; ss; eauto.
-      i.
-      hexploit MAYDIFF; eauto. i.
-      ii. exploit H.
-      { destruct id0 as [[]]; eauto.
-        inv MEM_EQUIV_SRC; solve_sem_idT.
-        rewrite -> LOCALS_EQ; eauto.
-      }
-      i. des.
-      esplits; eauto.
-      destruct id0 as [[]]; eauto.
-      inv MEM_EQUIV_TGT;
-        solve_sem_idT; rewrite <- LOCALS_EQ; eauto.
-    + econs; ss; eauto.
-      inv MEM_EQUIV_SRC.
-      inv MEM_EQUIV_TGT.
-      eapply mem_inject_change; eauto.
-  - inv MEM.
-    exploit forget_memory_unary_sound2; try exact SRC; eauto. i. des.
-    exploit forget_memory_unary_sound2; try exact TGT; eauto. i. des.
-    splits.
-    + econs; ss; eauto.
-      i.
-      hexploit MAYDIFF; eauto. i.
-      ii. exploit H.
-      { destruct id0 as [[]]; eauto.
-        inv MEM_EQUIV_SRC; solve_sem_idT.
-        rewrite -> LOCALS_EQ; eauto.
-      }
-      i. des.
-      esplits; eauto.
-      destruct id0 as [[]]; eauto.
-      inv MEM_EQUIV_TGT;
-        solve_sem_idT; rewrite <- LOCALS_EQ; eauto.
-    + econs; ss; eauto.
-      inv MEM_EQUIV_SRC.
-      inv MEM_EQUIV_TGT.
-      eapply mem_inject_change; eauto.
-Admitted.
+(*   - inv MEM. *)
+(*     exploit forget_memory_unary_sound1; try exact SRC; eauto. i. des. *)
+(*     exploit forget_memory_unary_sound2; try exact TGT; eauto. i. des. *)
+(*     splits. *)
+(*     + econs; ss; eauto. *)
+(*       i. *)
+(*       hexploit MAYDIFF; eauto. i. *)
+(*       ii. exploit H. *)
+(*       { destruct id0 as [[]]; eauto. *)
+(*         inv MEM_EQUIV_SRC; solve_sem_idT. *)
+(*         rewrite -> LOCALS_EQ; eauto. *)
+(*       } *)
+(*       i. des. *)
+(*       esplits; eauto. *)
+(*       destruct id0 as [[]]; eauto. *)
+(*       inv MEM_EQUIV_TGT; *)
+(*         solve_sem_idT; rewrite <- LOCALS_EQ; eauto. *)
+(*     + econs; ss; eauto. *)
+(*       inv MEM_EQUIV_SRC. *)
+(*       inv MEM_EQUIV_TGT. *)
+(*       eapply mem_inject_change; eauto. *)
+(*   - inv MEM. *)
+(*     exploit forget_memory_unary_sound2; try exact SRC; eauto. i. des. *)
+(*     exploit forget_memory_unary_sound1; try exact TGT; eauto. i. des. *)
+(*     splits. *)
+(*     + econs; ss; eauto. *)
+(*       i. *)
+(*       hexploit MAYDIFF; eauto. i. *)
+(*       ii. exploit H. *)
+(*       { destruct id0 as [[]]; eauto. *)
+(*         inv MEM_EQUIV_SRC; solve_sem_idT. *)
+(*         rewrite -> LOCALS_EQ; eauto. *)
+(*       } *)
+(*       i. des. *)
+(*       esplits; eauto. *)
+(*       destruct id0 as [[]]; eauto. *)
+(*       inv MEM_EQUIV_TGT; *)
+(*         solve_sem_idT; rewrite <- LOCALS_EQ; eauto. *)
+(*     + econs; ss; eauto. *)
+(*       inv MEM_EQUIV_SRC. *)
+(*       inv MEM_EQUIV_TGT. *)
+(*       eapply mem_inject_change; eauto. *)
+(*   - inv MEM. *)
+(*     exploit forget_memory_unary_sound2; try exact SRC; eauto. i. des. *)
+(*     exploit forget_memory_unary_sound2; try exact TGT; eauto. i. des. *)
+(*     splits. *)
+(*     + econs; ss; eauto. *)
+(*       i. *)
+(*       hexploit MAYDIFF; eauto. i. *)
+(*       ii. exploit H. *)
+(*       { destruct id0 as [[]]; eauto. *)
+(*         inv MEM_EQUIV_SRC; solve_sem_idT. *)
+(*         rewrite -> LOCALS_EQ; eauto. *)
+(*       } *)
+(*       i. des. *)
+(*       esplits; eauto. *)
+(*       destruct id0 as [[]]; eauto. *)
+(*       inv MEM_EQUIV_TGT; *)
+(*         solve_sem_idT; rewrite <- LOCALS_EQ; eauto. *)
+(*     + econs; ss; eauto. *)
+(*       inv MEM_EQUIV_SRC. *)
+(*       inv MEM_EQUIV_TGT. *)
+(*       eapply mem_inject_change; eauto. *)
+(* Admitted. *)
