coq/def/TODO.v
@@ -409,3 +409,15 @@ Proof.
   - specialize (IHxs H).
     destruct (x_eq_dec x a) eqn:T; ss.
 Qed.
+
+Lemma list_forallb2_spec A (P1 P2: A -> A -> bool) l1 l2
+      (COND: list_forallb2 P1 l1 l2 = true)
+      (INC: forall a1 a2, P1 a1 a2 = true -> P2 a1 a2 = true)
+  : list_forallb2 P2 l1 l2 = true.
+Proof.
+  revert l2 COND.
+  induction l1; ss.
+  i. destruct l2; ss.
+  apply andb_true_iff in COND. des.
+  apply andb_true_iff. eauto.
+Qed.
