coq/proof/SoundPostcondCmd.v
@@ -53,15 +53,42 @@ Proof.
 Qed.
 
 (* TODO: move this *)
+
+Lemma AtomSetImpl_spec_aux x l s
+  : x `in` fold_left (flip add) l s <-> In x l \/ x `in` s.
+Proof.
+  split.
+  - revert x s.
+    induction l; eauto.
+    i. ss.
+    exploit IHl; eauto. i.
+    unfold flip in *.
+    des; eauto.
+    rewrite -> AtomSetFacts.add_iff in *. des; eauto.
+  - revert x s.
+    induction l; i.
+    + ss. des; done.
+    + ss. des; (exploit IHl; [|eauto]); eauto;
+            right; apply AtomSetFacts.add_iff; eauto.
+Qed.
+  
 Lemma AtomSetImpl_from_list_spec1 x l
   : AtomSetImpl.In x (AtomSetImpl_from_list l) <-> In x l.
 Proof.
-Admitted.
+  assert (EQUIV: In x l <-> In x l \/ x `in` empty).
+  { split; eauto.
+    i. des; eauto.
+    apply AtomSetFacts.empty_iff in H. done.
+  }
+  rewrite EQUIV.
+  apply AtomSetImpl_spec_aux.
+Qed.
 
 Lemma AtomSetImpl_from_list_spec2 x l
   : ~ AtomSetImpl.In x (AtomSetImpl_from_list l) <-> ~ In x l.
 Proof.
-Admitted.
+  split; ii; apply AtomSetImpl_from_list_spec1 in H0; done.
+Qed.
 
 Lemma AtomSetImpl_singleton_mem_false x y
   : AtomSetImpl.mem x (AtomSetImpl_from_list [y]) = false -> x <> y.
@@ -143,33 +170,17 @@ Admitted.
 
 Lemma step_equiv_except_mem
       conf st0 st1 evt
-      cmd cmds invst
+      cmd cmds
       (NONCALL: Instruction.isCallInst cmd = false)
       (CMDS: CurCmds st0.(EC) = cmd :: cmds)
       (STEP: sInsn conf st0 st1 evt)
-  : state_equiv_except_mem conf
-                           (monad.mbind _ _ (ptr_to_genericvalue conf (mkState st1.(EC) st1.(ECS) st0.(Mem)) invst) (Cmd.get_def_memory cmd))
-                           (mkState st1.(EC) st1.(ECS) st0.(Mem)) st1.
+  : exists mc,
+    <<MEM_CH_REL:mem_change_rel conf st0 mc cmd>> /\
+    <<STATE_EQUIV: state_equiv_except_mem conf (mkState st1.(EC) st1.(ECS) st0.(Mem)) st1 mc>>.
 Proof.
-    inv STEP; ss.
-    { econs.
-      - ss.
-      - ss.
-        i. (* TODO: malloc and mload *)
-        admit.
-    }
-    { econs.
-      - ss.
-      - ss. i.
-        unfold mload in *. des_ifs.
-        (* mload after free: use Memory.Mem.load_alloc_other. *)
-        admit.
-    }
-    { admit. (* mload after alloca *)
-    }
-    { admit. (* mload after store *) }
-    { inv CMDS. ss. }
-Admitted.
+  inv STEP; destruct cmd; inv CMDS; ss;
+    try by esplits; eauto; econs; eauto; econs; eauto.
+Qed.
 
 Lemma step_unique_preserved_mem
       conf st0 st1 evt
@@ -191,11 +202,212 @@ Proof.
   { admit. (* load after store *) }
 Admitted.
 
+Lemma mem_change_rel_state_transition
+      conf st0 st1 evt cmd cmds mc
+      (CMD: CurCmds (EC st0) = cmd :: cmds)
+      (NONCALL: Instruction.isCallInst cmd = false)
+      (STEP: sInsn conf st0 st1 evt)
+      (MEM_CH_rel: mem_change_rel conf st0 mc cmd)
+  : mem_change_rel2 conf {| EC := EC st1; ECS := ECS st1; Mem := Mem st0 |} mc cmd.
+Proof.
+  destruct cmd; ss;
+    inv STEP; ss;
+      des; esplits; eauto.
+Qed.
+
+Ltac exploit_inject_value :=
+  repeat (match goal with
+       | [H1: Invariant.inject_value ?inv ?vt1 ?vt2 = true |- _] =>
+         exploit InvState.Rel.inject_value_spec; try exact H1; eauto; clear H1
+       end;
+       (try by
+           match goal with
+           | [H: getOperandValue (CurTargetData ?conf) ?v (Locals (EC ?st)) (Globals ?conf) = Some ?gv1 |-
+              InvState.Unary.sem_valueT ?conf ?st ?invst (ValueT.lift Tag.physical ?v) = Some ?gv2] =>
+             destruct v; [ss; unfold IdT.lift; solve_sem_idT; eauto | ss]
+           end); i; des).
+
+Ltac inv_conf :=
+  match goal with
+  | [H: InvState.valid_conf ?m_src ?m_tgt ?conf_src ?conf_tgt |- _] =>
+    let TD := fresh in
+    let GL := fresh in
+    destruct H as [[TD GL]]; rewrite TD in *; rewrite GL in *
+  end.
+
+Ltac inject_clarify :=
+  repeat
+    match goal with
+    | [H1: getTypeAllocSize ?TD ?ty = Some ?tsz1,
+           H2: getTypeAllocSize ?TD ?ty = Some ?tsz2 |- _] =>
+      rewrite H1 in H2; inv H2
+    | [H: proj_sumbool ?dec = true |- _] =>
+      destruct dec; ss; subst
+    | [H1: getOperandValue (CurTargetData ?conf) ?v (Locals (EC ?st)) ?GL = Some ?gv1,
+           H2: InvState.Unary.sem_valueT ?conf ?st ?invst (ValueT.lift Tag.physical ?v) =
+               Some ?gv2 |- _] =>
+      let Hnew := fresh in
+      assert (Hnew: InvState.Unary.sem_valueT conf st invst (ValueT.lift Tag.physical v) = Some gv1);
+      [ destruct v; [ss; unfold IdT.lift; solve_sem_idT; eauto | ss] | ];
+      rewrite Hnew in H2; clear Hnew; inv H2
+    | [H1: getOperandValue (CurTargetData ?conf) (value_id ?x) (Locals (EC ?st)) ?GL = Some ?gv1 |-
+       InvState.Unary.sem_idT ?st ?invst (Tag.physical, ?x) = Some ?gv2] =>
+      let Hnew := fresh in
+      assert (Hnew: InvState.Unary.sem_idT st invst (Tag.physical, x) = Some gv1); [ss|];
+      apply Hnew; clear Hnew
+    end.
+
+Lemma inject_event_implies_mem_change_inject
+      m_src conf_src st0_src mc_src cmd_src
+      m_tgt conf_tgt st0_tgt mc_tgt cmd_tgt
+      invst0 invmem0 inv0
+      (CONF: InvState.valid_conf m_src m_tgt conf_src conf_tgt)
+      (STATE : InvState.Rel.sem conf_src conf_tgt st0_src st0_tgt invst0 invmem0 inv0)
+      (MEM : InvMem.Rel.sem conf_src conf_tgt (Mem st0_src) (Mem st0_tgt) invmem0)
+      (INJECT: postcond_cmd_inject_event cmd_src cmd_tgt inv0 = true)
+      (MEM_CH_REL_SRC: mem_change_rel conf_src st0_src mc_src cmd_src)
+      (MEM_CH_REL_TGT: mem_change_rel conf_tgt st0_tgt mc_tgt cmd_tgt)
+  : mem_change_inject conf_src conf_tgt invmem0 mc_src mc_tgt.
+Proof.
+  destruct cmd_src; destruct cmd_tgt; ss;
+    (try by des; subst; econs); des; subst; simtac;
+      (try by exploit_inject_value; inv_conf; inject_clarify; econs; eauto).
+  unfold Invariant.is_private in *. des_ifs.
+  destruct x as [t x]; unfold ValueT.lift in *. des_ifs.
+  inv STATE. inv SRC.
+  exploit PRIVATE.
+  { apply IdTSet.mem_2; eauto. }
+  { inv_conf.
+    inject_clarify.
+  }
+  i. des_ifs.
+  econs; eauto.
+Qed.
+
+(* TODO: move *)
+
+
+Lemma inject_value_monotone
+      v1 def_mem_src def_src use_src
+      v2 def_mem_tgt def_tgt use_tgt
+      inv0
+      (INJECT: Invariant.inject_value
+                 (ForgetMemory.t def_mem_src def_mem_tgt
+                                 (Forget.t def_src def_tgt use_src use_tgt inv0)) v1 v2)
+  : Invariant.inject_value inv0 v1 v2.
+Proof.
+  eapply inject_value_forget_monotone; eauto.
+  eapply inject_value_forget_memory_monotone; eauto.
+Qed.
+
+Lemma postcond_cmd_check_monotone
+      cmd_src cmd_tgt inv0
+      (COND : postcond_cmd_check
+                cmd_src cmd_tgt
+                (AtomSetImpl_from_list (Cmd.get_def cmd_src))
+                (AtomSetImpl_from_list (Cmd.get_def cmd_tgt))
+                (AtomSetImpl_from_list (Cmd.get_ids cmd_src))
+                (AtomSetImpl_from_list (Cmd.get_ids cmd_tgt))
+                (ForgetMemory.t (Cmd.get_def_memory cmd_src) (Cmd.get_def_memory cmd_tgt)
+                                (Forget.t (AtomSetImpl_from_list (Cmd.get_def cmd_src))
+                                          (AtomSetImpl_from_list (Cmd.get_def cmd_tgt))
+                                          (AtomSetImpl_from_list (Cmd.get_leaked_ids cmd_src))
+                                          (AtomSetImpl_from_list (Cmd.get_leaked_ids cmd_tgt)) inv0)) = true)
+  : postcond_cmd_check
+      cmd_src cmd_tgt
+      (AtomSetImpl_from_list (Cmd.get_def cmd_src))
+      (AtomSetImpl_from_list (Cmd.get_def cmd_tgt))
+      (AtomSetImpl_from_list (Cmd.get_ids cmd_src))
+      (AtomSetImpl_from_list (Cmd.get_ids cmd_tgt))
+      inv0 = true.
+Proof.
+  unfold postcond_cmd_check in *.
+  des_ifs.
+  clear -Heq1 Heq2.
+  rename Heq1 into INJECT_F. rename Heq2 into INJECT_T.
+  apply negb_false_iff in INJECT_T.
+  apply negb_true_iff in INJECT_F.
+  destruct cmd_src; destruct cmd_tgt; ss.
+  - apply ExprPairSet.exists_2 in INJECT_T; try by solve_compat_bool.
+    inv INJECT_T. des.
+    apply ExprPairSet.filter_1 in H; try by solve_compat_bool.
+    exploit ExprPairSet.exists_1; try by solve_compat_bool.
+    unfold ExprPairSet.Exists.
+    esplits; eauto.
+  - simtac.
+    inject_clarify.
+    rewrite andb_true_r in *.
+    exploit inject_value_forget_monotone; eauto.
+  - simtac.
+    exploit inject_value_monotone; eauto.
+  - simtac.
+    inject_clarify.
+    rewrite andb_true_r in *.
+    exploit inject_value_forget_monotone; eauto.
+  - simtac.
+    inject_clarify.
+    rewrite andb_true_r in *.
+    exploit inject_value_forget_monotone; eauto.
+  - unfold Invariant.is_private in *. des_ifs.
+    + ss. unfold ForgetMemory.unary in *.
+      des_ifs; ss;
+        unfold Forget.unary in *;
+        rewrite IdTSetFacts.filter_b in INJECT_T; try by solve_compat_bool; clarify.
+    + ss.
+      rewrite IdTSetFacts.filter_b in INJECT_T; try by solve_compat_bool; clarify.
+  - simtac.
+    repeat solve_des_bool; clarify.
+    + exploit inject_value_monotone; try exact H2; eauto.
+    + exploit inject_value_monotone; try exact H0; eauto.
+  - simtac.
+    + solve_des_bool.
+      * exploit inject_value_forget_monotone; eauto.
+      * exploit list_forallb2_spec.
+        { apply H0. }
+        { instantiate
+            (1:=(fun p1 p2 => let
+                     '(_, attr1, v1) := p1 in
+                   let
+                     '(_, attr2, v2) := p2 in
+                   attributes_dec attr1 attr2 &&
+                   Invariant.inject_value inv0
+                   (ValueT.lift Tag.physical v1) (ValueT.lift Tag.physical v2))).
+          i. ss.
+          destruct a1. destruct a2.
+          destruct p. destruct p0.
+          simtac.
+          exploit inject_value_forget_monotone; eauto. i.
+          des_ifs.
+        }
+        i. clarify.
+    + solve_des_bool.
+      * exploit inject_value_forget_monotone; eauto.
+      * exploit list_forallb2_spec.
+        { apply H0. }
+        { instantiate
+            (1:=(fun p1 p2 => let
+                     '(_, attr1, v1) := p1 in
+                   let
+                     '(_, attr2, v2) := p2 in
+                   attributes_dec attr1 attr2 &&
+                   Invariant.inject_value inv0
+                   (ValueT.lift Tag.physical v1) (ValueT.lift Tag.physical v2))).
+          i. ss.
+          destruct a1. destruct a2.
+          destruct p. destruct p0.
+          simtac.
+          exploit inject_value_forget_monotone; eauto. i.
+          des_ifs.
+        }
+        i. clarify.
+Qed.
+
 Lemma postcond_cmd_sound
-      conf_src st0_src cmd_src cmds_src
-      conf_tgt st0_tgt cmd_tgt cmds_tgt
+      m_src conf_src st0_src cmd_src cmds_src
+      m_tgt conf_tgt st0_tgt cmd_tgt cmds_tgt
       invst0 invmem0 inv0
       st1_tgt evt inv1
+      (CONF: InvState.valid_conf m_src m_tgt conf_src conf_tgt)
       (POSTCOND: Postcond.postcond_cmd cmd_src cmd_tgt inv0 = Some inv1)
       (STATE: InvState.Rel.sem conf_src conf_tgt st0_src st0_tgt invst0 invmem0 inv0)
       (MEM: InvMem.Rel.sem conf_src conf_tgt st0_src.(Mem) st0_tgt.(Mem) invmem0)
@@ -233,9 +445,16 @@ Proof.
   { inv STATE. inv SRC. hexploit step_unique_preserved_except; try exact CMDS_SRC; eauto. }
   { inv STATE. inv TGT. hexploit step_unique_preserved_except; try exact CMDS_TGT; eauto. }
   intro STATE_FORGET. des.
+  hexploit step_equiv_except_mem; try exact NONCALL_SRC; eauto. i. des.
+  hexploit step_equiv_except_mem; try exact NONCALL_TGT; eauto. i. des.
   exploit forget_memory_sound; try exact STATE_FORGET; eauto.
-  { hexploit step_equiv_except_mem; try exact NONCALL_SRC; eauto. }
-  { hexploit step_equiv_except_mem; try exact NONCALL_TGT; eauto. }
+  { eapply mem_change_rel_state_transition; eauto. }
+  { eapply mem_change_rel_state_transition; eauto. }
+  { exploit inject_event_implies_mem_change_inject; try exact STATE; eauto.
+    exploit postcond_cmd_check_monotone; eauto. i.
+    unfold postcond_cmd_check in *. des_ifs.
+    apply negb_false_iff. eauto.
+  }
   { inv STATE_FORGET.
     hexploit step_unique_preserved_mem; try exact NONCALL_SRC; inv SRC; eauto.
     apply forget_unique_leak_disjoint.
